theories/semtyping.v
@@ -1,10 +1,21 @@
-Require Import join normalform imports.
+Require Import conv par geq imports.
 
-Definition ProdSpace (PA : tm -> Prop) (PF : tm -> (tm -> Prop) -> Prop) (b : tm) :=
-  forall a PB, PA a -> PF a PB -> PB (tApp b a).
+Module Type lr_sig
+  (Import lattice : Lattice)
+  (Import syntax : syntax_sig lattice)
+  (Import par : par_sig lattice syntax)
+  (Import ieq : geq_sig lattice syntax)
+  (Import conv : conv_sig lattice syntax par ieq).
 
-Definition SumSpace (PA : tm -> Prop) (PF : tm -> (tm -> Prop) -> Prop) t :=
-  (exists a b, t ⇒* tPack a b /\ PA a /\ (forall PB, PF a PB -> PB b)) \/ wne t.
+Module pfacts := par_facts lattice syntax par.
+Import pfacts.
+
+Module cfacts := conv_facts lattice syntax par ieq conv.
+Import cfacts.
+
+Definition ProdSpace Ξ ℓ0 (PA : T -> tm -> Prop) (PF : tm -> (T -> tm -> Prop) -> Prop)ℓ (b : tm) :=
+  IOk Ξ ℓ b /\
+  forall a PB, PA ℓ0 a -> PF a PB -> PB ℓ (tApp b ℓ0 a).
 
 (* Logical Relation:
 
@@ -18,56 +29,39 @@ Definition SumSpace (PA : tm -> Prop) (PF : tm -> (tm -> Prop) -> Prop) t :=
 
  *)
 
-Reserved Notation "⟦ A ⟧ i , I ↘ S" (at level 70).
-Inductive InterpExt i (I : nat -> tm -> Prop) : tm -> (tm -> Prop) -> Prop :=
-| InterpExt_Ne A : ne A -> ⟦ A ⟧ i , I ↘ wne
-| InterpExt_Nat : ⟦ tNat ⟧ i , I ↘ (fun a => exists v, a ⇒* v /\ is_nat_val v)
-| InterpExt_Fun A B PA PF :
-  ⟦ A ⟧ i , I ↘ PA ->
-  (forall a, PA a -> exists PB, PF a PB) ->
-  (forall a PB, PF a PB -> ⟦ B[a..] ⟧ i , I ↘ PB) ->
-  ⟦ tPi A B ⟧ i , I ↘ (ProdSpace PA PF)
+
+Inductive InterpExt Ξ i (I : nat -> tm -> Prop) : tm -> (T -> tm -> Prop) -> Prop :=
+| InterpExt_Fun ℓ0 A B PA PF :
+  InterpExt Ξ i I A PA ->
+  (forall a, PA ℓ0 a -> exists PB, PF a PB) ->
+  (forall a PB, PA ℓ0 a -> PF a PB -> InterpExt Ξ i I B[a..] PB) ->
+  InterpExt Ξ i I (tPi ℓ0 A B) (ProdSpace Ξ ℓ0 PA PF)
 | InterpExt_Univ j :
   j < i ->
-  ⟦ tUniv j ⟧ i , I ↘ (I j)
-| InterpExt_Eq a b A :
-  nf a ->
-  nf b ->
-  nf A ->
-   ⟦ tEq a b A ⟧ i , I ↘ (fun p => (p ⇒* tRefl /\ Coherent a b) \/ wne p)
-| InterpExt_Sig A B PA PF :
-  ⟦ A ⟧ i , I ↘ PA ->
-  (forall a, PA a -> exists PB, PF a PB) ->
-  (forall a PB, PF a PB -> ⟦ B[a..] ⟧ i , I ↘ PB) ->
-  ⟦ tSig A B ⟧ i , I ↘ SumSpace PA PF
+  InterpExt Ξ i I (tUniv j) (fun ℓ A => IOk Ξ ℓ A /\  I j A)
 | InterpExt_Step A A0 PA :
   (A ⇒ A0) ->
-  ⟦ A0 ⟧ i , I ↘ PA ->
-  ⟦ A ⟧ i , I ↘ PA
-where "⟦ A ⟧ i , I ↘ S" := (InterpExt i I A S).
+  InterpExt Ξ i I A0 PA ->
+  InterpExt Ξ i I A PA.
+Notation " ⟦ Ξ ⊨ A ⟧ i ; I ↘ S" := (InterpExt Ξ i I A S)
+                                     (at level 70, no associativity).
 
-Lemma InterpExt_Eq' i I PA a b A :
-  nf a ->
-  nf b ->
-  nf A ->
-  PA = (fun p => (p ⇒* tRefl /\ Coherent a b) \/ wne p) ->
-  ⟦ tEq a b A ⟧ i , I ↘ PA.
-Proof. hauto lq:on use:InterpExt_Eq. Qed.
+Equations InterpUnivN (Ξ : econtext) (n : nat) : tm -> (T -> tm -> Prop) -> Prop
+  by wf n lt :=
+  InterpUnivN Ξ n := InterpExt Ξ n
+                       (fun m A =>
+                          match Compare_dec.lt_dec m n with
+                          | left h => exists PA, InterpUnivN Ξ m A PA
+                          | right _ => False
+                          end).
+Notation " ⟦ Ξ ⊨ A ⟧ i  ↘ S" := (InterpUnivN Ξ i A S)
+                                  (at level 70, no associativity).
 
-Lemma InterpExt_Univ' i I j PF :
-  PF = I j ->
+Lemma InterpExt_Univ' i Ξ I j PF :
+  PF = (fun ℓ A => IOk Ξ ℓ A /\  I j A) ->
   j < i ->
-  ⟦ tUniv j ⟧ i , I ↘ PF.
+  InterpExt Ξ i I (tUniv j) PF.
 Proof. hauto lq:on ctrs:InterpExt. Qed.
-
-Equations InterpUnivN (n : nat) : tm -> (tm -> Prop) -> Prop by wf n lt :=
-  InterpUnivN n := InterpExt n (fun m A =>
-                                  match Compare_dec.lt_dec m n with
-                                  | left h => exists PA, InterpUnivN m A PA
-                                  | right _ => False
-                                  end).
-
-Notation "⟦ A ⟧ i ↘ S" := (InterpUnivN i A S) (at level 70).
 
 (* ---------------------------------------------------- *)
 
@@ -76,9 +70,9 @@ Notation "⟦ A ⟧ i ↘ S" := (InterpUnivN i A S) (at level 70).
    simplify the unfolding above to just mention InterpUnivN
    without doing the case analysis.
 *)
-Lemma InterpExt_lt_redundant i I A PA
-  (h : ⟦ A ⟧ i , I ↘ PA) :
-       ⟦ A ⟧ i , (fun j A =>
+Lemma InterpExt_lt_redundant i Ξ I A PA
+  (h : ⟦ Ξ ⊨ A ⟧ i ; I ↘ PA) :
+       ⟦ Ξ ⊨ A ⟧ i ; (fun j A =>
                      match Compare_dec.lt_dec j i with
                      | left h => I j A
                      | right _ => False
@@ -86,38 +80,38 @@ Lemma InterpExt_lt_redundant i I A PA
 Proof.
   elim : A PA / h.
   - hauto lq:on ctrs:InterpExt.
-  - hauto l:on.
-  - hauto l:on ctrs:InterpExt.
+  (* - hauto l:on. *)
+  (* - hauto l:on ctrs:InterpExt. *)
   - move => m h.
     apply InterpExt_Univ' => //.
     case : Compare_dec.lt_dec => //.
   - hauto l:on ctrs:InterpExt.
-  - hauto l:on ctrs:InterpExt.
-  - hauto l:on ctrs:InterpExt.
+  (* - hauto l:on ctrs:InterpExt. *)
+  (* - hauto l:on ctrs:InterpExt. *)
 Qed.
 
-Lemma InterpExt_lt_redundant2 i I A PA
- (h : ⟦ A ⟧ i , (fun j A =>
+Lemma InterpExt_lt_redundant2 Ξ i I A PA
+ (h : ⟦ Ξ ⊨ A ⟧ i ; (fun j A =>
                       match Compare_dec.lt_dec j i with
                      | left h => I j A
                      | right _ => False
                      end) ↘ PA) :
-  ⟦ A ⟧ i , I ↘ PA.
+  ⟦ Ξ ⊨ A ⟧ i ; I ↘ PA.
 Proof.
   elim : A PA / h.
   - hauto lq:on ctrs:InterpExt.
-  - hauto l:on.
-  - hauto l:on ctrs:InterpExt.
+  (* - hauto l:on. *)
+  (* - hauto l:on ctrs:InterpExt. *)
   - move => m ?.
     apply InterpExt_Univ' => //.
     case : Compare_dec.lt_dec => //.
   - hauto l:on ctrs:InterpExt.
-  - hauto l:on ctrs:InterpExt.
-  - hauto lq:on ctrs:InterpExt.
+  (* - hauto l:on ctrs:InterpExt. *)
+  (* - hauto lq:on ctrs:InterpExt. *)
 Qed.
 
-Lemma InterpUnivN_nolt i :
-  InterpUnivN i = InterpExt i (fun j A => exists PA, ⟦ A ⟧ j ↘ PA).
+Lemma InterpUnivN_nolt Ξ i :
+  InterpUnivN Ξ i = InterpExt Ξ i (fun j A => exists PA, ⟦ Ξ ⊨ A ⟧ j ↘ PA).
 Proof.
   simp InterpUnivN.
   fext => A P.
@@ -127,39 +121,38 @@ Qed.
 
 #[export]Hint Rewrite InterpUnivN_nolt : InterpUniv.
 
-Lemma InterpExt_Fun_inv i I A B P
-  (h :  ⟦ tPi A B ⟧ i , I ↘ P) :
-  exists (PA : tm -> Prop) (PF : tm -> (tm -> Prop) -> Prop),
-     ⟦ A ⟧ i , I ↘ PA /\
-    (forall a, PA a -> exists PB, PF a PB) /\
-    (forall a PB, PF a PB -> ⟦ B[a..] ⟧ i , I ↘ PB) /\
-    P = ProdSpace PA PF.
+Lemma InterpExt_Fun_inv Ξ i I ℓ0 A B P
+  (h :  ⟦ Ξ ⊨ tPi ℓ0 A B ⟧ i ; I ↘ P) :
+  exists (PA : T -> tm -> Prop) (PF : tm -> (T -> tm -> Prop) -> Prop),
+     ⟦ Ξ ⊨ A ⟧ i ; I ↘ PA /\
+    (forall a, PA ℓ0 a -> exists PB, PF a PB) /\
+    (forall a PB, PA ℓ0 a -> PF a PB -> ⟦ Ξ ⊨ B[a..] ⟧ i ; I ↘ PB) /\
+    P = ProdSpace Ξ ℓ0 PA PF.
 Proof.
-  move E : (tPi A B) h => T h.
+  move E : (tPi ℓ0 A B) h => T h.
   move : A B E.
   elim : T P / h => //.
   - hauto q:on inv:tm.
-  - hauto l:on.
-  - move => *; subst.
-    hauto lq:on inv:Par ctrs:InterpExt use:Par_subst.
+  (* - hauto l:on. *)
+  - hauto lq:on rew:off inv:Par ctrs:InterpExt use:Par_subst.
 Qed.
 
-Lemma InterpExt_Sig_inv i I A B P
-  (h :  ⟦ tSig A B ⟧ i , I ↘ P) :
-  exists (PA : tm -> Prop) (PF : tm -> (tm -> Prop) -> Prop),
-     ⟦ A ⟧ i , I ↘ PA /\
-    (forall a, PA a -> exists PB, PF a PB) /\
-    (forall a PB, PF a PB -> ⟦ B[a..] ⟧ i , I ↘ PB) /\
-    P = SumSpace PA PF.
-Proof.
-  move E : (tSig A B) h => T h.
-  move : A B E.
-  elim : T P / h => //.
-  - hauto q:on inv:tm.
-  - hauto l:on.
-  - move => *; subst.
-    hauto lq:on inv:Par ctrs:InterpExt use:Par_subst.
-Qed.
+(* Lemma InterpExt_Sig_inv i I A B P *)
+(*   (h :  ⟦ tSig A B ⟧ i , I ↘ P) : *)
+(*   exists (PA : tm -> Prop) (PF : tm -> (tm -> Prop) -> Prop), *)
+(*      ⟦ A ⟧ i , I ↘ PA /\ *)
+(*     (forall a, PA a -> exists PB, PF a PB) /\ *)
+(*     (forall a PB, PF a PB -> ⟦ B[a..] ⟧ i , I ↘ PB) /\ *)
+(*     P = SumSpace PA PF. *)
+(* Proof. *)
+(*   move E : (tSig A B) h => T h. *)
+(*   move : A B E. *)
+(*   elim : T P / h => //. *)
+(*   - hauto q:on inv:tm. *)
+(*   - hauto l:on. *)
+(*   - move => *; subst. *)
+(*     hauto lq:on inv:Par ctrs:InterpExt use:Par_subst. *)
+(* Qed. *)
 
 (* For all of the proofs about InterpUnivN below, we need to
    do them in two steps. Once for InterpExt, and then tie the
@@ -168,38 +161,37 @@ Qed.
 (* -----  I-PiAlt is admissible (free of PF, the relation R on paper)  ---- *)
 
 
-Lemma InterpUnivN_Fun_nopf i A B PA :
-  ⟦ A ⟧ i ↘ PA ->
-  (forall a, PA a -> exists PB, ⟦ B[a..] ⟧ i ↘ PB) ->
-  ⟦ tPi A B ⟧ i ↘ (ProdSpace PA (fun a PB => ⟦ B[a..] ⟧ i ↘ PB)).
+Lemma InterpUnivN_Fun_nopf Ξ i ℓ0 A B PA :
+  ⟦ Ξ ⊨ A ⟧ i ↘ PA ->
+  (forall a, PA ℓ0 a -> exists PB, ⟦ Ξ ⊨ B[a..] ⟧ i ↘ PB) ->
+  ⟦ Ξ ⊨ tPi ℓ0 A B ⟧ i ↘ (ProdSpace Ξ ℓ0 PA (fun a PB => ⟦ Ξ ⊨ B[a..] ⟧ i ↘ PB)).
 Proof.
   hauto l:on ctrs:InterpExt rew:db:InterpUniv.
 Qed.
 
-Lemma InterpUnivN_Sig_nopf i A B PA :
-  ⟦ A ⟧ i ↘ PA ->
-  (forall a, PA a -> exists PB, ⟦ B[a..] ⟧ i ↘ PB) ->
-  ⟦ tSig A B ⟧ i ↘ (SumSpace PA (fun a PB => ⟦ B[a..] ⟧ i ↘ PB)).
-Proof.
-  hauto l:on ctrs:InterpExt rew:db:InterpUniv.
-Qed.
+(* Lemma InterpUnivN_Sig_nopf i A B PA : *)
+(*   ⟦ A ⟧ i ↘ PA -> *)
+(*   (forall a, PA a -> exists PB, ⟦ B[a..] ⟧ i ↘ PB) -> *)
+(*   ⟦ tSig A B ⟧ i ↘ (SumSpace PA (fun a PB => ⟦ B[a..] ⟧ i ↘ PB)). *)
+(* Proof. *)
+(*   hauto l:on ctrs:InterpExt rew:db:InterpUniv. *)
+(* Qed. *)
 
 (* --------------- relation is cumulative ----------------- *)
 
-
-Lemma InterpExt_cumulative i j I A PA :
+Lemma InterpExt_cumulative Ξ i j I A PA :
   i <= j ->
-   ⟦ A ⟧ i , I ↘ PA ->
-   ⟦ A ⟧ j , I ↘ PA.
+   ⟦ Ξ ⊨ A ⟧ i ; I ↘ PA ->
+   ⟦ Ξ ⊨ A ⟧ j ; I ↘ PA.
 Proof.
   move => h h0.
   elim : A PA /h0;
     hauto l:on ctrs:InterpExt use:PeanoNat.Nat.le_trans.
 Qed.
 
-Lemma InterpUnivN_cumulative i A PA :
-   ⟦ A ⟧ i ↘ PA -> forall j, i <= j ->
-   ⟦ A ⟧ j ↘ PA.
+Lemma InterpUnivN_cumulative Ξ i A PA :
+   ⟦ Ξ ⊨ A ⟧ i ↘ PA -> forall j, i <= j ->
+   ⟦ Ξ ⊨ A ⟧ j ↘ PA.
 Proof.
   hauto l:on rew:db:InterpUniv use:InterpExt_cumulative.
 Qed.
@@ -209,184 +201,167 @@ Qed.
 (* The logical relation is closed under parallel reduction,
    forwards and backwards. *)
 
-Lemma InterpExt_preservation i I A B P (h : ⟦ A ⟧ i , I ↘ P) :
+Lemma InterpExt_preservation Ξ i I A B P (h : ⟦ Ξ ⊨ A ⟧ i ; I ↘ P) :
   (A ⇒ B) ->
-  ⟦ B ⟧ i , I ↘ P.
+  ⟦ Ξ ⊨ B ⟧ i ; I ↘ P.
 Proof.
   move : B.
   elim : A P / h; auto.
-  - hauto lq:on ctrs:InterpExt db:nfne.
-  - hauto lq:on inv:Par ctrs:InterpExt.
-  - move => A B PA PF hPA ihPA hPB hPB' ihPB T hT.
+  (* - hauto lq:on ctrs:InterpExt db:nfne. *)
+  (* - hauto lq:on inv:Par ctrs:InterpExt. *)
+  - move => ℓ0 A B PA PF hPA ihPA hPB hPB' ihPB T hT.
     elim /Par_inv :  hT => //.
-    move => hPar A0 A1 B0 B1 h0 h1 [? ?] ?; subst.
+    move => hPar ℓ1 A0 A1 B0 B1 h0 h1 [? ? ?] ?; subst.
     apply InterpExt_Fun; auto.
-    move => a PB hPB0.
+    move => a PB ha hPB0.
     apply : ihPB; eauto.
     sfirstorder use:Par_cong, Par_refl.
   - hauto lq:on inv:Par ctrs:InterpExt.
-  - move => a b A  ? ? ? B.
-    elim /Par_inv=>// h ? ? ? a0 b0 A0 ? ? ? [] *. subst.
-    apply InterpExt_Eq'; eauto with nfne.
-    fext => p.
-    f_equal.
-    apply propositional_extensionality.
-    hauto lq:on use:Par_Coherent, Coherent_transitive, Coherent_symmetric.
-  - move => A B PA PF hPA ihPA hPB hPB' ihPB T hT.
-    elim /Par_inv :  hT => //.
-    move => hPar A0 A1 B0 B1 h0 h1 [? ?] ?; subst.
-    apply InterpExt_Sig; auto.
-    move => a PB hPB0.
-    apply : ihPB; eauto.
-    sfirstorder use:Par_cong, Par_refl.
+  (* - move => a b A  ? ? ? B. *)
+  (*   elim /Par_inv=>// h ? ? ? a0 b0 A0 ? ? ? [] *. subst. *)
+  (*   apply InterpExt_Eq'; eauto with nfne. *)
+  (*   fext => p. *)
+  (*   f_equal. *)
+  (*   apply propositional_extensionality. *)
+  (*   hauto lq:on use:Par_Coherent, Coherent_transitive, Coherent_symmetric. *)
+  (* - move => A B PA PF hPA ihPA hPB hPB' ihPB T hT. *)
+  (*   elim /Par_inv :  hT => //. *)
+  (*   move => hPar A0 A1 B0 B1 h0 h1 [? ?] ?; subst. *)
+  (*   apply InterpExt_Sig; auto. *)
+  (*   move => a PB hPB0. *)
+  (*   apply : ihPB; eauto. *)
+  (*   sfirstorder use:Par_cong, Par_refl. *)
   - move => A B P h0 h1 ih1 C hC.
     have [D [h2 h3]] := Par_confluent _ _ _ h0 hC.
     hauto lq:on ctrs:InterpExt.
 Qed.
 
 
-Lemma InterpUnivN_preservation i A B P (h : ⟦ A ⟧ i ↘ P) :
+Lemma InterpUnivN_preservation Ξ i A B P (h : ⟦ Ξ ⊨ A ⟧ i ↘ P) :
   (A ⇒ B) ->
-  ⟦ B ⟧ i ↘ P.
+  ⟦ Ξ ⊨ B ⟧ i ↘ P.
 Proof. hauto l:on rew:db:InterpUnivN use: InterpExt_preservation. Qed.
 
-Lemma InterpExt_back_preservation_star i I A B P (h : ⟦ B ⟧ i , I ↘ P) :
+Lemma InterpExt_back_preservation_star Ξ i I A B P (h : ⟦ Ξ ⊨ B ⟧ i ; I ↘ P) :
   A ⇒* B ->
-  ⟦ A ⟧ i , I ↘ P.
+  ⟦ Ξ ⊨ A ⟧ i ; I ↘ P.
 Proof. induction 1; hauto l:on ctrs:InterpExt. Qed.
 
-Lemma InterpExt_preservation_star i I A B P (h : ⟦ A ⟧ i , I ↘ P) :
+Lemma InterpExt_preservation_star Ξ i I A B P (h : ⟦ Ξ ⊨ A ⟧ i ; I ↘ P) :
   A ⇒* B ->
-  ⟦ B ⟧ i , I ↘ P.
+  ⟦ Ξ ⊨ B ⟧ i ; I ↘ P.
 Proof. induction 1; hauto l:on use:InterpExt_preservation. Qed.
 
-Lemma InterpUnivN_preservation_star i A B P (h : ⟦ A ⟧ i ↘ P) :
+Lemma InterpUnivN_preservation_star Ξ i A B P (h : ⟦ Ξ ⊨ A ⟧ i ↘ P) :
   A ⇒* B ->
-  ⟦ B ⟧ i ↘ P.
+  ⟦ Ξ ⊨ B ⟧ i ↘ P.
 Proof. hauto l:on rew:db:InterpUnivN use:InterpExt_preservation_star. Qed.
 
-Lemma InterpUnivN_back_preservation_star i A B P (h : ⟦ B ⟧ i ↘ P) :
+Lemma InterpUnivN_back_preservation_star Ξ i A B P (h : ⟦ Ξ ⊨ B ⟧ i ↘ P) :
   A ⇒* B ->
-  ⟦ A ⟧ i ↘ P.
+  ⟦ Ξ ⊨ A ⟧ i ↘ P.
 Proof. hauto l:on rew:db:InterpUnivN use:InterpExt_back_preservation_star. Qed.
-
-(* ---------------------------------------------------------- *)
-
-Lemma InterpUnivN_Coherent i A B P (h : ⟦ B ⟧ i ↘ P) :
-  Coherent A B ->
-  ⟦ A ⟧ i ↘ P.
-Proof.
-  hauto l:on unfold:Coherent use:InterpUnivN_back_preservation_star, InterpUnivN_preservation_star.
-Qed.
 
 (* ---------------------------------------------------------- *)
 (* inversion lemmas for InterpExt. To invert the InterpExt
    judgment, we have to be careful about the step case. *)
 
-Lemma InterpExt_Ne_inv i I A P :
-  ne A ->
-  ⟦ A ⟧ i , I ↘ P ->
-  P = wne.
-Proof.
-  move => + h0.
-  elim : A P /h0 =>//.
-  hauto l:on inv:- db:nfne.
-Qed.
+(* Lemma InterpExt_Ne_inv Ξ i I A P : *)
+(*   ne A -> *)
+(*   ⟦ Ξ ⊨ A ⟧ i ; I ↘ P -> *)
+(*   P = wne. *)
+(* Proof. *)
+(*   move => + h0. *)
+(*   elim : A P /h0 =>//. *)
+(*   hauto l:on inv:- db:nfne. *)
+(* Qed. *)
 
-Lemma InterpExt_Nat_inv i I P :
-  ⟦ tNat ⟧ i , I ↘ P ->
-  P = fun a => exists v, a ⇒* v /\ is_nat_val v.
-Proof.
-  move E : tNat => A h.
-  move : E.
-  elim : A P / h; hauto q:on inv:tm,Par.
-Qed.
+(* Lemma InterpExt_Nat_inv i I P : *)
+(*   ⟦ tNat ⟧ i , I ↘ P -> *)
+(*   P = fun a => exists v, a ⇒* v /\ is_nat_val v. *)
+(* Proof. *)
+(*   move E : tNat => A h. *)
+(*   move : E. *)
+(*   elim : A P / h; hauto q:on inv:tm,Par. *)
+(* Qed. *)
 
-Lemma InterpExt_Univ_inv i I P j :
-  ⟦ tUniv j ⟧ i , I ↘ P ->
-  P = I j /\ j < i.
+Lemma InterpExt_Univ_inv Ξ i I P j :
+  ⟦ Ξ ⊨ tUniv j ⟧ i ; I ↘ P ->
+  P = (fun ℓ A => IOk Ξ ℓ A /\  I j A) /\ j < i.
 Proof.
   move E : (tUniv j) => A h.
   move : E.
   elim : A P / h; hauto q:on rew:off inv:Par,tm.
 Qed.
 
-Lemma InterpUnivN_Ne_inv i A P :
-  ne A ->
-  ⟦ A ⟧ i ↘ P ->
-  P = wne.
-Proof.
-  sfirstorder use:InterpExt_Ne_inv rew:db:InterpUniv.
-Qed.
+(* Lemma InterpUnivN_Ne_inv i A P : *)
+(*   ne A -> *)
+(*   ⟦ A ⟧ i ↘ P -> *)
+(*   P = wne. *)
+(* Proof. *)
+(*   sfirstorder use:InterpExt_Ne_inv rew:db:InterpUniv. *)
+(* Qed. *)
 
-Lemma InterpUnivN_Nat_inv i P :
-  ⟦ tNat ⟧ i ↘ P ->
-  P = fun a => exists v, a ⇒* v /\ (is_nat_val v).
-Proof. hauto l:on rew:db:InterpUnivN use:InterpExt_Nat_inv. Qed.
+(* Lemma InterpUnivN_Nat_inv i P : *)
+(*   ⟦ tNat ⟧ i ↘ P -> *)
+(*   P = fun a => exists v, a ⇒* v /\ (is_nat_val v). *)
+(* Proof. hauto l:on rew:db:InterpUnivN use:InterpExt_Nat_inv. Qed. *)
 
-Lemma InterpExt_Eq_inv i I a b A P :
-  ⟦ tEq a b A ⟧ i , I ↘ P ->
-  (P = fun A => A ⇒* tRefl /\ Coherent a b \/ wne A) /\ wn a /\ wn b /\ wn A.
-Proof.
-  move E : (tEq a b A) => T h.
-  move : a b A E.
-  elim : T P /h => //.
-  hauto q:on inv:tm.
-  hauto lq:on ctrs:rtc.
-  move => A A0 PA hred hA0 ih a b A1 ?. subst.
-  elim /Par_inv : hred=>//.
-  move => hred ? ? ? a2 b2 A2 ? ? ? [] *;subst.
-  split; last by hauto lq:on rew:off ctrs:rtc.
-  specialize ih with (1 := eq_refl).
-  move : ih => [->] *.
-  fext => A. do 2 f_equal.
-  apply propositional_extensionality.
-  hauto lq:on use:Par_Coherent, Coherent_symmetric, Coherent_transitive.
-Qed.
+(* Lemma InterpExt_Eq_inv i I a b A P : *)
+(*   ⟦ tEq a b A ⟧ i , I ↘ P -> *)
+(*   (P = fun A => A ⇒* tRefl /\ Coherent a b \/ wne A) /\ wn a /\ wn b /\ wn A. *)
+(* Proof. *)
+(*   move E : (tEq a b A) => T h. *)
+(*   move : a b A E. *)
+(*   elim : T P /h => //. *)
+(*   hauto q:on inv:tm. *)
+(*   hauto lq:on ctrs:rtc. *)
+(*   move => A A0 PA hred hA0 ih a b A1 ?. subst. *)
+(*   elim /Par_inv : hred=>//. *)
+(*   move => hred ? ? ? a2 b2 A2 ? ? ? [] *;subst. *)
+(*   split; last by hauto lq:on rew:off ctrs:rtc. *)
+(*   specialize ih with (1 := eq_refl). *)
+(*   move : ih => [->] *. *)
+(*   fext => A. do 2 f_equal. *)
+(*   apply propositional_extensionality. *)
+(*   hauto lq:on use:Par_Coherent, Coherent_symmetric, Coherent_transitive. *)
+(* Qed. *)
 
-Lemma InterpUnivN_Eq_inv i a b A P :
-  ⟦ tEq a b A ⟧ i ↘ P ->
-  P = (fun p => (p ⇒* tRefl /\ Coherent a b) \/ wne p) /\ wn a /\ wn b /\ wn A.
-Proof.
-  simp InterpUniv.
-  hauto l:on use:InterpExt_Eq_inv.
-Qed.
+(* Lemma InterpUnivN_Eq_inv i a b A P : *)
+(*   ⟦ tEq a b A ⟧ i ↘ P -> *)
+(*   P = (fun p => (p ⇒* tRefl /\ Coherent a b) \/ wne p) /\ wn a /\ wn b /\ wn A. *)
+(* Proof. *)
+(*   simp InterpUniv. *)
+(*   hauto l:on use:InterpExt_Eq_inv. *)
+(* Qed. *)
 
 (* ------------- relation is deterministic ---------------- *)
 
-Lemma InterpExt_deterministic i I A PA PB :
-  ⟦ A ⟧ i , I ↘ PA ->
-  ⟦ A ⟧ i , I ↘ PB ->
+Lemma InterpExt_deterministic Ξ i I A PA PB :
+  ⟦ Ξ ⊨ A ⟧ i ; I ↘ PA ->
+  ⟦ Ξ ⊨ A ⟧ i ; I ↘ PB ->
   PA = PB.
 Proof.
   move => h.
   move : PB.
   elim : A PA / h.
-  - hauto lq:on inv:InterpExt ctrs:InterpExt use:InterpExt_Ne_inv.
-  - hauto lq:on inv:InterpExt use:InterpExt_Nat_inv.
-  - move => A B PA PF hPA ihPA hPB hPB' ihPB P hP.
+  (* - hauto lq:on inv:InterpExt ctrs:InterpExt use:InterpExt_Ne_inv. *)
+  (* - hauto lq:on inv:InterpExt use:InterpExt_Nat_inv. *)
+  - move => ℓ0 A B PA PF hPA ihPA hPB hPB' ihPB P hP.
     move /InterpExt_Fun_inv : hP.
     intros (PA0 & PF0 & hPA0 & hPB0 & hPB0' & ?); subst.
     have ? : PA0 = PA by sfirstorder. subst.
-    fext => b a PB ha.
+    rewrite /ProdSpace.
+    fext => *.
     apply propositional_extensionality.
     hauto lq:on rew:off.
   - hauto lq:on rew:off inv:InterpExt ctrs:InterpExt use:InterpExt_Univ_inv.
-  - hauto lq:on inv:InterpExt use:InterpExt_Eq_inv.
-  - move => A B PA PF hPA ihPA hPB hPB' ihPB P hP.
-    move /InterpExt_Sig_inv : hP.
-    intros (PA0 & PF0 & hPA0 & hPB0 & hPB0' & ?); subst.
-    have ? : PA0 = PA by sfirstorder. subst.
-    rewrite /SumSpace.
-    fext => t.
-    apply propositional_extensionality.
-    hauto lq:on rew:off.
   - hauto l:on use:InterpExt_preservation.
 Qed.
 
-Lemma InterpUnivN_deterministic i A PA PB :
-  ⟦ A ⟧ i ↘ PA ->
-  ⟦ A ⟧ i ↘ PB ->
+Lemma InterpUnivN_deterministic Ξ i A PA PB :
+  ⟦ Ξ ⊨ A ⟧ i ↘ PA ->
+  ⟦ Ξ ⊨ A ⟧ i ↘ PB ->
   PA = PB.
 Proof.
   simp InterpUnivN. apply InterpExt_deterministic.
@@ -395,9 +370,9 @@ Qed.
 (* slight generalization to work with any levels using cumulativity. *)
 
 
-Lemma InterpExt_deterministic' i j I A PA PB :
-   ⟦ A ⟧ i , I ↘ PA ->
-   ⟦ A ⟧ j , I ↘ PB ->
+Lemma InterpExt_deterministic' Ξ i j I A PA PB :
+   ⟦ Ξ ⊨ A ⟧ i ; I ↘ PA ->
+   ⟦ Ξ ⊨ A ⟧ j ; I ↘ PB ->
   PA = PB.
 Proof.
   move => h0 h1.
@@ -406,30 +381,75 @@ Proof.
   - move => ?. have : j <= i by lia. hauto l:on use:InterpExt_cumulative, InterpExt_deterministic.
 Qed.
 
-Lemma InterpUnivN_deterministic' i j  A PA PB :
-  ⟦ A ⟧ i ↘ PA ->
-  ⟦ A ⟧ j ↘ PB ->
+Lemma InterpUnivN_deterministic' Ξ i j  A PA PB :
+  ⟦ Ξ ⊨ A ⟧ i ↘ PA ->
+  ⟦ Ξ ⊨ A ⟧ j ↘ PB ->
   PA = PB.
 Proof. hauto lq:on rew:off use:InterpExt_deterministic' rew:db:InterpUniv. Qed.
 
+(* ------ Elements from the interpreted set are all well-graded --- *)
+Lemma InterpExt_Ok Ξ i I A PA :
+  InterpExt Ξ i I A PA -> forall ℓ a, PA ℓ a -> IOk Ξ ℓ a.
+Proof.
+  move => h.
+  elim : A PA / h.
+  - hauto lq:on.
+  - sfirstorder.
+  - sfirstorder.
+Qed.
+
+Lemma InterpExt_IEq Ξ i I A PA (h : InterpExt Ξ i I A PA) :
+  forall ℓ B, IEq Ξ ℓ A B ->
+  InterpExt Ξ i I B PA.
+Proof.
+  elim : A PA / h.
+  - move => ℓ0 A B PA PF hPA ihPA hTot hRes ihPF ℓ1 T.
+    elim /IEq_inv=>// _ ? A0 A1 B0 B1 h0 h1 [*]. subst.
+    apply InterpExt_Fun; eauto.
+    move => a PB hPF ha.
+    apply : ihPF; eauto.
+    apply : ifacts.ieq_morphing_iok; eauto.
+    rewrite /elookup.
+    case => //=. hauto l:on use:InterpExt_Ok.
+    move => n ℓ2 ?.
+    apply : IO_Var; eauto.
+    apply lattice.meet_idempotent.
+  - hauto lq:on inv:IEq ctrs:InterpExt.
+  - hauto q:on use:simulation ctrs:InterpExt.
+Qed.
+
+
 (* ----- Improved inversion lemma for functions (Pi Inv Alt) ---------- *)
 
-
-Lemma InterpExt_Fun_inv_nopf i I A B P  (h : InterpExt i I (tPi A B) P) :
-  exists (PA : tm -> Prop),
-     ⟦ A ⟧ i , I ↘ PA /\
-    (forall a, PA a -> exists PB, ⟦ B[a..] ⟧ i , I ↘ PB) /\
-      P = ProdSpace PA (fun a PB => ⟦ B[a..] ⟧ i , I ↘ PB).
+Lemma InterpExt_Fun_inv_nopf Ξ i I ℓ0 A B P  (h : InterpExt Ξ i I (tPi ℓ0 A B) P) :
+  exists PA,
+     ⟦ Ξ ⊨ A ⟧ i ; I ↘ PA /\
+    (forall a, PA ℓ0 a -> exists PB, ⟦ Ξ ⊨ B[a..] ⟧ i ; I ↘ PB) /\
+      P = ProdSpace Ξ ℓ0 PA (fun a PB => ⟦ Ξ ⊨ B[a..] ⟧ i ; I ↘ PB).
 Proof.
   move /InterpExt_Fun_inv : h. intros (PA & PF & hPA & hPF & hPF' & ?); subst.
   exists PA. repeat split => //.
   - sfirstorder.
-  - fext => b a PB ha.
+  - fext => b a.
     apply propositional_extensionality.
+    rewrite /ProdSpace.
+    have : forall (A B C : Prop), (B <-> C) -> (A /\ B  <-> A /\ C) by tauto.
+    apply.
     split.
-    + move  : hPF ha . move /[apply]. intros (PB0 & hPB0). move => *.
-      have ? : PB0 = PB by eauto using InterpExt_deterministic. sfirstorder.
+    + move => h a0 PB /[dup] ?.
+      move : hPF . move /[apply]. intros (PB0 & hPB0). move => *.
+      have ? : PB0 = PB by eauto using InterpExt_deterministic.
+      sfirstorder.
     + sfirstorder.
+Qed.
+
+(* ---------------------------------------------------------- *)
+
+Lemma InterpUnivN_Conv Ξ i A B P (h : ⟦ Ξ ⊨ B ⟧ i ↘ P) :
+  conv Ξ A B ->
+  ⟦ Ξ ⊨ A ⟧ i ↘ P.
+Proof.
+  hauto l:on unfold:Coherent use:InterpUnivN_back_preservation_star, InterpUnivN_preservation_star.
 Qed.
 
 
